Started structuring development to relate LTS simulation and trace inclusion.

LTS.thy
@@ -4,36 +4,50 @@ imports Main
 
 begin
 
-section {* Labelled transition systems *}
+section {* Execution models *}
+
+subsection {* Labeled transition systems *}
 
 text {* The semantics of a B component is a discrete, eventful, state-transition systems. We 
 first define what is meant exactly by such systems. Any system is, at a given time in a state. 
 Conversely, a system has a set of possible states. A system evolves from state to state,
-and such changes called transitions. Also when a system makes a transition, this is observable
-and this observation is called an event. State, transition and event are three different
-entities and a type is declared for each: *}
+and such changes called transitions. The following record definition of 
+@{text "('st, 'ev) Transition}"} models transitions, where the parametric sorts @{text "'st"} 
+and @{text "'ev"} represent states and events, respectively. *}
 
-record ('st, 'ev) Transition =
-  src :: 'st
-  dst :: 'st
-  lbl :: 'ev
-  
+record ('st, 'ev) Tr =
+  src :: 'st -- "source state"
+  dst :: 'st -- "destination state"
+  lbl :: 'ev -- "labeling event"
+
+text {* Building on this formalization of transitions, the record @{text "('st, 'ev) LTS"} 
+formalizes labeled transition systems (LTS):  *}
+
 record ('st, 'ev) LTS =
-  init :: "'st set" (* a set of initial states *)
-  trans :: "('st, 'ev) Transition set" (* a set of transitions *)
-  
+  init :: "'st set" -- "set of initial states"
+  trans :: "('st, 'ev) Tr set" -- "set of transitions"
+
+text {* The inductively defined set @{term "states"} yields the reachable states of a 
+given LTS. *}
+
 inductive_set states :: "('st, 'ev) LTS \<Rightarrow> 'st set" for m :: "('st, 'ev) LTS" where
   base[elim!]: "s \<in> init m \<Longrightarrow> s \<in> states m"
 | step[elim!]: "\<lbrakk> t \<in> trans m; src t \<in> states m \<rbrakk> \<Longrightarrow> dst t \<in> states m"
-  
-definition successors :: "('st, 'ev) LTS \<Rightarrow> 'st set \<Rightarrow> 'st set" where
-"successors lts S \<equiv> { s | s . \<exists> t \<in> trans lts. src t \<in> S \<and> dst t = s}"
   
 text {* A few lemmas related to reachable states are then enunciated and proved. 
 First, all the initial states are reachable states:*}
 
 lemma reachable_init: "init m \<subseteq> states m" 
   by auto
+
+text {* Next, the successors states of the reachable states are themselves reachable states.
+We first define a function @{text "successors"} that returns the set of successors of a
+given set @{text "S"} of states in a given LTS @{text "L"}: *}
+
+definition successors :: "('st, 'ev) LTS \<Rightarrow> 'st set \<Rightarrow> 'st set" where
+"successors L S \<equiv> { s | s . \<exists> t \<in> trans L. src t \<in> S \<and> dst t = s}"
+
+text {* Next, we show that the successors of the reachable states are also reachable. *}
 
 lemma reachable_stable: "successors m (states m) \<subseteq> states m"
   unfolding successors_def by auto
@@ -61,41 +75,85 @@ proof
   qed
 qed
 
-text {* Next we enunciate and prove a similar lemma for predicates. *}
+text {* Next we enunciate and prove a similar lemma for predicates. In a LTS @{text "L"}, 
+if every initial state
+statisfies some predicate @{text "P"} and, for each transition, whenever the source state
+satisfies @{text "P"}, the destination state also satisfies @{text "P"}, then all the
+reachable states satisfy @{text "P"} (and this is an invariant of the LTS). *}
 lemma reachable_induct_predicate:
-  assumes base: "\<forall> s \<in> init m . p s" and 
-          step: "\<forall> t \<in> trans m . p (src t) \<longrightarrow> p (dst t)"
-  shows "\<forall> s \<in> (states m) . p s"
+  assumes base: "\<forall> s \<in> init L . P s" and 
+          step: "\<forall> t \<in> trans L . P (src t) \<longrightarrow> P (dst t)"
+  shows "\<forall> s \<in> (states L) . P s"
 proof
   fix x
-  assume "x \<in> states m" 
-  thus "p x"
+  assume "x \<in> states L" 
+  thus "P x"
   proof (induct x)
     fix i
-    assume "i \<in> init m"
-    with base show "p i" ..
+    assume "i \<in> init L"
+    with base show "P i" ..
   next
     fix t
-    assume "t \<in> trans m" "src t \<in> states m" "p (src t)"
-    with step show "p (dst t)" unfolding successors_def by auto
+    assume "t \<in> trans L" "src t \<in> states L" "P (src t)"
+    with step show "P (dst t)" unfolding successors_def by auto
   qed
 qed
 
 subsection {* Behavior *}
 
-text {* Internal behavior. *}
+subsubsection {* Internal behaviour *}
 
-inductive_set runs :: "('st, 'ev) LTS \<Rightarrow> ('st, 'ev) Transition list set"  
-          for m :: "('st, 'ev) LTS" where
-  base: "[] : runs m"
-| one[elim!]: "\<lbrakk> t \<in> trans m; src t \<in> init m \<rbrakk> \<Longrightarrow> [t] \<in> runs m"
-| step[elim!]: "\<lbrakk> t \<in> trans m; r \<in> runs m; r \<noteq> []; src t = dst (last r) \<rbrakk> \<Longrightarrow> r @ [t] \<in> runs m"
+text {* Two views of behavior are formalized. The first view is the internal behavior, and
+corresponds to the set of possible executions. An execution is a sequence of transitions, such
+that two consecutive transitions have coincident state. We introduce the abbreviation @{text "Run"}
+to name the type for executions: *}
 
-text {* External behavior. *}
+type_synonym ('st, 'ev) Run = "('st, 'ev) Tr list"
 
-definition traces :: "('st, 'ev) LTS \<Rightarrow> 'ev list set" where
-  "traces m \<equiv> { map lbl r | r . r \<in> runs m }"
+text {* The inductive set @{text "runs"}
+denotes all possible executions of a given LTS @{text "L"}. There are two base cases, 
+corresponding to the empty execution and to executions with a single transition: *}
+
+inductive_set runs :: "('st, 'ev) LTS \<Rightarrow> ('st, 'ev) Run set"  
+          for L :: "('st, 'ev) LTS" where
+  base: "[] \<in> runs L"
+| start: "\<lbrakk> t \<in> trans L; src t \<in> init L \<rbrakk> \<Longrightarrow> [t] \<in> runs L"
+| step: "\<lbrakk> t \<in> trans L; r \<noteq> []; r \<in> runs L; src t = dst (last r) \<rbrakk> \<Longrightarrow> r @ [t] \<in> runs L"
+
+inductive_cases empty_run : "[] \<in> runs m"
+inductive_cases one_step_run : "[t] \<in> runs m"
+inductive_cases multi_step_run : "r @ [t] \<in> runs m"
+
+lemma 
+assumes "t \<in> trans L \<and> src t \<in> init L"
+shows "[t] \<in> runs L"
+by (metis assms runs.start)
+
+text {* The following lemma states that for any run $r$ of a LTS $m$, such that $r$ is not the 
+empty run, then the source state of the first transition is an initial state of $m$. *}
+
+lemma "r \<in> runs m \<Longrightarrow> r \<noteq> [] \<Longrightarrow> src(hd r) \<in> init m"
+proof(induct rule: runs.induct, auto)
+qed
+
+subsubsection {* External behavior. *}
+
+text {* The external, or observable, behavior of a LTS is restricted to the events labeling its 
+transitions. We give the name @{text "Trace"} to the type of event lists: *}
+
+type_synonym 'ev Trace = "'ev list"
+
+text {* We define the \emph{trace} of a run to be the sequence of events along that run: *}
+
+fun "trace_of_run" :: "('st, 'ev) Run \<Rightarrow> 'ev Trace" 
+where
+"trace_of_run [] = []" |
+"trace_of_run (t # ts) = (lbl t) # (trace_of_run ts)"
+
+text {* We then define the \emph{traces} of an LTS from the corresponding runs: *}
+
+definition traces :: "('st, 'ev) LTS \<Rightarrow> 'ev Trace set" where
+  "traces m \<equiv> { trace_of_run r | r . r \<in> runs m }"
 
 end
-
 
