Simulation.thy
@@ -3,34 +3,59 @@ theory Simulation
 imports Main LTS
 
 begin
-section {* Behaviour: a set of traces *}
+section {* Relating LTSes: simulation *}
 
-text {* We introduce the notion of simulation: a relation between the states of one LTS
+subsection {* Basic definitions *}
+
+text {* We formalize the notion of simulation on LTSes. Classic definitions of simulation
+often consider a single LTS, and simulation is established between two states of the same
+LTS. Here, a simulation is a relation @{text "r"} between the states of one LTS
 and the states of another LTS such that any transition taken by the former can be simulated
-by the latter, i.e. the latter can follow a transition that is labeled with the same event,
-and leads to a state where it can continue the simulation: *}
+by the latter. 
+
+The relation between states is the basis of a relation between transitions:
+the source and destinations must be pairwise related, and the label shall coincide. This
+is formalized in the function @{text "sim_transition"} *}
+
+definition sim_transition :: "'st rel \<Rightarrow> ('st, 'ev) Tr \<Rightarrow> ('st, 'ev) Tr \<Rightarrow> bool"
+where "sim_transition r t t' \<equiv> (src t, src t') \<in> r \<and> lbl t = lbl t' \<and> (dst t, dst t') \<in> r"
+
+text {* The former transition used to extend the notion of simulation to the set of
+transitions of two LTSes @{text "l1"} and @{text "l2"}. This is specified in the function 
+@{text "sim_trans"}: *}
+
+definition sim_trans :: "'st rel \<Rightarrow> ('st, 'ev) LTS \<Rightarrow> ('st, 'ev) LTS \<Rightarrow> bool" where
+  "sim_trans r l l' \<equiv> 
+    \<forall> s s' . (s, s') \<in> r \<longrightarrow>
+      (\<forall> t \<in> trans l . src t = s \<longrightarrow>
+        (\<exists> t' \<in> trans l' . src t' = s' \<and> sim_transition r t t'))"
+
+text {* Another condition to establish a simulation between @{text "l"} and @{text "l'"}, is that 
+every initial state of the former must be related to an initial state of the latter by @{text "s"}: *}
 
 definition simulation_init :: "'st rel \<Rightarrow> ('st, 'ev) LTS \<Rightarrow> ('st, 'ev) LTS \<Rightarrow> bool" where
-  "simulation_init r l1 l2 \<equiv> \<forall> s1 \<in> init l1 . \<exists> s2 \<in> init l2 . (s1, s2) \<in> r"
+  "simulation_init r l l' \<equiv> \<forall> s \<in> init l . \<exists> s' \<in> init l' . (s, s') \<in> r"
 
-definition simulation_step :: "'st rel \<Rightarrow> ('st, 'ev) LTS \<Rightarrow> ('st, 'ev) LTS \<Rightarrow> bool" where
-  "simulation_step r l1 l2 \<equiv> 
-    \<forall> s1 s2 . (s1, s2) \<in> r \<longrightarrow>
-      (\<forall> t1 \<in> trans l1 . src t1 = s1 \<longrightarrow>
-        (\<exists> t2 \<in> trans l2 . src t2 = s2 \<and> lbl t1 = lbl t2 \<and> (dst t1, dst t2) \<in> r))"
+text {* We are now equiped to give the characterize that a relation @{text "r"} defines a simulation 
+of @{text "l"} by @{text "l'"}: *}
 
 definition simulation :: "'st rel \<Rightarrow> ('st, 'ev) LTS \<Rightarrow> ('st, 'ev) LTS \<Rightarrow> bool" where
-  "simulation r l1 l2 \<equiv> simulation_init r l1 l2 \<and> simulation_step r l1 l2"
+  "simulation r l l' \<equiv> simulation_init r l l' \<and> sim_trans r l l'"
+
+text {* Based on the notion of simulation, we introduce the relation simulates on LTS: *}
+definition simulates :: "('st, 'ev) LTS \<Rightarrow> ('st, 'ev) LTS \<Rightarrow> bool" (infixl "\<sim>" 50) where
+  "(l1 \<sim> l2) \<equiv> \<exists> r . simulation r l2 l1"
+
+subsection {* Properties *}
 
 text {* Let us verify some basic properties of simulations. First we have that the
 identity relation establishes that a LTS simulates itself. *}
-  (* maybe use Id_on (states l) instead of Id ? *)
-lemma simulation_identity : "simulation Id l l" 
-  unfolding simulation_def simulation_init_def simulation_step_def by auto
 
-text {* Second, we have that the composition of two simulation relations 
-is a simulation relation. *}
-lemma simulation_transitivity:
+lemma simulation_identity : "simulation Id l l" 
+  unfolding simulation_def simulation_init_def sim_trans_def sim_transition_def by auto
+
+text {* Second, we have that the composition of two simulation relations is a simulation relation. *}
+lemma simulation_closed:
 assumes s12: "simulation r12 l1 l2" and s23: "simulation r23 l2 l3"
 shows "simulation (r12 O r23) l1 l3"
 proof -
@@ -40,17 +65,13 @@ proof -
   by simp metis
 moreover
   from s12 s23
-  have "simulation_step (r12 O r23) l1 l3"
-  unfolding simulation_step_def simulation_def relcomp_unfold
+  have "sim_trans (r12 O r23) l1 l3"
+  unfolding sim_trans_def simulation_def sim_transition_def relcomp_unfold
   by simp metis
   ultimately show ?thesis unfolding simulation_def ..
 qed
 
 text {* Next we carry these properties over to the simulates relation over LTS. *}
-
-text {* Based on the notion of simulation, we introduce the relation simulates on LTS: *}
-definition simulates :: "('st, 'ev) LTS \<Rightarrow> ('st, 'ev) LTS \<Rightarrow> bool" (infixl "\<sim>" 50) where
-  "(l1 \<sim> l2) \<equiv> \<exists> r . simulation r l2 l1"
 
 lemma simulates_reflexivity: "l \<sim> l" 
   unfolding simulates_def
@@ -69,8 +90,89 @@ moreover
   from s12 obtain r where "simulation r l2 l1" unfolding simulates_def ..
 ultimately
   have "simulation (s O r) l3 l1" 
-    by (rule simulation_transitivity[of "s" "l3" "l2" "r" "l1"])
+    by (rule simulation_closed[of "s" "l3" "l2" "r" "l1"])
   then show ?thesis unfolding simulates_def by auto
 qed
+
+subsection {* Simulation and behavior *}
+
+text {* The predicate @{text "sim_run"} defines when a state relation @{text "r"} establishes 
+  a simulation between two runs *}
   
+inductive sim_run :: "'st rel \<Rightarrow> ('st, 'ev) Run \<Rightarrow> ('st, 'ev) Run \<Rightarrow> bool"
+where
+  "sim_run s [] []"
+| "sim_transition s t1 t2 \<Longrightarrow> sim_run s [t1] [t2]"
+| "ts1 \<noteq> [] \<and> ts2 \<noteq> [] \<and> sim_run s ts1 ts2 \<and> 
+   sim_transition s t1 t2 \<and> dst t1 = src(hd ts1) \<and> dst t2 = src(hd ts2) \<Longrightarrow> 
+   sim_run s (t1 # ts1) (t2 # ts2)"
+
+text {* An important property on simulation and runs is that if a relation @{text "s"}
+establishes a simulation of a run @{text "r"} with a run @{text "r'"}, then 
+@{text "r"} and @{text "r'"} are exhibit the same observable behavior: *}
+
+theorem "sim_run s r r' \<Longrightarrow> trace_of_run r = trace_of_run r'"
+proof(induct rule: sim_run.induct, simp, unfold sim_transition_def, simp, simp)
+qed
+
+lemma sim_run_empty_iff: "sim_run s r r' \<Longrightarrow> (r = [] \<longleftrightarrow> r' = [])"
+proof(induct rule: sim_run.induct, simp, simp, simp)
+qed
+
+lemma "sim_run s r r' \<and> r = [] \<Longrightarrow> r' = []"
+by (metis sim_run_empty_iff)
+
+lemma sim_run_last_trans: "sim_run s r r' \<Longrightarrow> r \<noteq> [] \<Longrightarrow> (dst(last r), dst(last r')) \<in> s"
+sorry
+
+lemma sim_run_app_trans: 
+  "sim_run s r r' \<Longrightarrow> r \<noteq> [] \<and> src t = dst(last r) \<and> src t' = dst(last r') \<and>
+  sim_transition s t t' \<Longrightarrow> sim_run s (r @ [t]) (r' @ [t'])"
+sorry
+
+text {* Next, we enunciate, and prove, the property that the existence of a simulation @{text "s"} 
+of the LTS @{text "l"} by the LTS @{text "l'"} guarantees that every run of the former may be 
+simulated with @{text "s"} by a run of the latter. *}
+
+lemma 
+  assumes sim: "simulation s l l'" 
+  shows "\<forall> r \<in> runs l . \<exists> r' \<in> runs l' . sim_run s r r'"
+proof
+  fix r
+  show "r \<in> runs l \<Longrightarrow> \<exists> r' \<in> runs l'. sim_run s r r'"
+  proof(induct rule: runs.induct, auto)
+    have "[] \<in> runs l' \<and> sim_run s [] []" by (simp add: runs.base sim_run.intros(1))
+    thus "\<exists> r' \<in> runs l'. sim_run s [] r'" by auto
+  next
+    fix t
+    assume step: "t \<in> trans l" and init: "src t \<in> init l"
+    with assms obtain s' where src: "(src t, s') \<in> s \<and> s' \<in> init l'" 
+      unfolding simulation_def simulation_init_def by blast
+    with step and assms obtain t' 
+      where t': "t' \<in> trans l' \<and> src t' = s' \<and> sim_transition s t t'"
+      unfolding simulation_def sim_trans_def by blast
+    with src have "[t'] \<in> runs l'" by (metis runs.start)
+    with t' have "[t'] \<in> runs l' \<and> sim_run s [t] [t']" by (metis sim_run.intros(2))
+    hence "\<exists> r' . r' \<in> runs l' \<and> sim_run s [t] r'" ..
+    thus "\<exists> r' \<in> runs l'. sim_run s [t] r'" by auto
+  next
+    fix t r x
+    assume h0: "t \<in> trans l" and h1: "r \<noteq> []" and h2: "r \<in> runs l" and h3: "src t = dst (last r)" and
+    h4: "x \<in> runs l'" and h5: "sim_run s r x"
+    with sim have h6: "x \<noteq> []" by (metis sim_run_empty_iff)
+    from h1 and h5 have h7: "(dst(last r), dst(last x)) \<in> s" by (metis sim_run_last_trans)
+    obtain s' where h8: "s' = dst(last x)" by blast
+    from h7 and h8 have h9: "(dst(last r), s') \<in> s" by simp
+    from sim h0 h3 h9 obtain t' where t': "t' \<in> trans l' \<and> src t' = s' \<and> sim_transition s t t'" 
+      unfolding simulation_def sim_trans_def by blast
+    from t' h4 h6 and h8 have h10: "x @ [t'] \<in> runs l'" by (metis runs.step)
+    from h1 h5 h6 h3 h8 t' have h11: "sim_run s (r @ [t]) (x @ [t'])" by (metis sim_run_app_trans)
+    from h10 and h11 have "x @ [t'] \<in> runs l' \<and> sim_run s (r @ [t]) (x @ [t'])" ..
+    hence "\<exists> r' . r' \<in> runs l' \<and> sim_run s (r @ [t]) r'" ..
+    thus "\<exists> r' \<in> runs l'. sim_run s (r @ [t]) r'" by auto
+  qed
+qed
+
 end
+
+
