TraceRefinement.thy
@@ -1,0 +1,25 @@
+theory TraceRefinement
+
+imports Main LTS Simulation
+
+begin
+
+definition refines :: "('st, 'ev) LTS \<Rightarrow> ('st, 'ev) LTS \<Rightarrow> bool" (infixl "\<sqsupseteq>" 50) 
+  where "lc \<sqsupseteq> la \<equiv> traces lc \<subseteq> traces la"
+
+abbreviation is_refined_by :: "('st, 'ev) LTS \<Rightarrow> ('st, 'ev) LTS \<Rightarrow> bool" (infixl "\<sqsubseteq>" 50) 
+  where "la \<sqsubseteq> lc \<equiv> lc \<sqsupseteq> la"
+
+lemma refines_refl: "l \<sqsupseteq> l" unfolding refines_def by auto
+  
+lemma lts_refines_trans: "l1 \<sqsupseteq> l2 \<and> l2 \<sqsupseteq> l3 \<Longrightarrow>  l1 \<sqsupseteq> l3" 
+  unfolding refines_def by auto
+
+(* TODO relate simulation and trace containment *)
+lemma "(l1 :: ('st, 'ev) LTS) \<sim> l2 \<Longrightarrow> \<forall> r2 \<in> runs l2 . \<exists> r . \<exists> r1 \<in> runs l1 . simulate_run r r2 r1"
+sorry
+
+theorem "l1 \<sim> l2 \<Longrightarrow> l1 \<sqsubseteq> l1"
+sorry
+
+end
