ROOT
@@ -1,0 +1,7 @@
+session "b-means" = "HOL" +
+  options [ quick_and_dirty = true, document = pdf, document_output = "output", document_variants="document:outline=/proof,/theory" ]
+  theories [document = false]
+    (* Foo Bar *)
+  theories
+    LTS Simulation TraceRefinement
+  files "document/root.tex"
